proof/invariant-abstract/RISCV64/ArchKHeap_AI.thy
@@ -302,7 +302,7 @@ lemma valid_vspace_objs_lift_weak:
 
 lemma translate_address_lift_weak:
   assumes aobj_at: "\<And>P P' p. vspace_obj_pred P' \<Longrightarrow> f \<lbrace>\<lambda>s. P (obj_at P' p s)\<rbrace>"
-  shows "f \<lbrace>\<lambda>s. P (translate_address pt_root vref s) \<rbrace>"
+  shows "f \<lbrace>\<lambda>s. P (translate_address pt_root vref (ptes_of s)) \<rbrace>"
   unfolding translate_address_def pt_lookup_target_def
   apply (clarsimp simp: comp_def obind_def)
   apply (rule hoare_lift_Pf2[where f=ptes_of, OF _ ptes_of_lift[OF aobj_at]]; simp)
@@ -648,17 +648,13 @@ lemma valid_vso_at_lift_aobj_at:
   apply assumption
   done *)
 
-lemma translate_address_pte_update:
-  "ptes_of (f s) = ptes_of s \<Longrightarrow> translate_address pt vref (f s) = translate_address pt vref s"
-  by (fastforce simp: translate_address_def pt_lookup_target_def obind_def split: option.split)
-
 lemma valid_global_vspace_mappings_arch_update[simp]:
   "\<lbrakk> riscv_global_pt (arch_state (f s)) = riscv_global_pt (arch_state s);
      riscv_kernel_vspace (arch_state (f s)) = riscv_kernel_vspace (arch_state s);
      ptes_of (f s) = ptes_of s \<rbrakk>
      \<Longrightarrow> valid_global_vspace_mappings (f s) = valid_global_vspace_mappings s"
   unfolding valid_global_vspace_mappings_def
-  by (simp add: translate_address_pte_update)
+  by simp
 
 lemma valid_table_caps_ptD:
   "\<lbrakk> caps_of_state s p = Some (ArchObjectCap (PageTableCap p' None));
